proof/Vector.v
@@ -1,0 +1,121 @@
+Require Import Coq.Arith.Arith.
+Parameter A : Set.
+
+Inductive vec : nat -> Set :=
+  | vnil : vec 0
+  | vcons : forall n, A -> vec n -> vec (S n).
+
+Definition hd : forall n, n > 0 -> vec n -> A.
+Proof.
+  intros n H v ; induction v.
+  elim (gt_irrefl _ H).
+  assumption.
+Defined.
+
+Definition tl : forall n, n > 0 -> vec n -> vec (pred n).
+Proof.
+  intros n H v ; induction v.
+  elim (gt_irrefl _ H).
+  simpl.
+  assumption.
+Defined.  
+
+Set Implicit Arguments.
+
+Definition nth : forall n m, m < n -> vec n -> A.
+Proof.
+  intros.
+  induction H0.
+  elim (lt_n_O _ H).
+  assumption.
+Defined.
+
+Require Import Omega.
+
+Definition vapp : forall n m, vec n -> vec m -> vec (n + m).
+Proof.
+  intros.
+  induction H.
+  simpl.
+  assumption.
+
+  pose (vcons (n + m) a IHvec).
+  assert(S (n + m) = S n + m).
+  simpl.
+  reflexivity.
+  rewrite <- H1.
+  exact v.
+Defined.
+
+Require Import Eqdep.
+
+Definition vec_plus : forall n m, forall t : vec (n + m), 
+  exists t' : vec (m + n), eq_dep nat vec (n + m) t (m + n) t'.
+Proof.
+  intros.
+  rewrite plus_comm.
+  exists t.
+  auto.
+Qed.
+
+Require Import JMeq.
+
+Lemma eq_dep_vnil : forall n, forall a : vec n,
+  n = 0 -> eq_dep nat vec n a 0 vnil.
+Proof.
+  intros.
+  
+  simpl.
+  induction a.
+  auto.
+
+  discriminate.
+Qed.
+
+Lemma eq_vnil : forall v : vec 0, v = vnil.
+Proof.
+  intros.
+  apply eq_dep_eq with (P := vec).
+  apply eq_dep_vnil.
+  auto.
+Qed.
+
+Lemma vapp_vnil_l : forall n, forall v : vec n,
+  vapp vnil v = v.
+Proof.
+  intros.
+  simpl.
+  reflexivity.
+Qed.
+
+Lemma vapp_vnil_dep_l : forall n, forall v : vec n,
+  eq_dep nat vec n (vapp vnil v) n v.
+Proof.
+  intros.
+  simpl.
+  apply eq_dep_intro.
+Qed.
+  
+Lemma vapp_vnil_dep_r : forall n, forall v : vec n,
+  eq_dep nat vec (n + 0) (vapp v vnil) n v.
+Proof.
+  intros.
+  induction v.
+  simpl ; auto.
+
+  simpl.
+
+  pose (proj2 (equiv_eqex_eqdep nat vec (n + 0) n (vapp v vnil) v) IHv).
+  dependent rewrite -> e.
+  simpl.
+  auto.
+Qed.
+
+Infix ":::" := vcons (at level 60, right associativity) : vector_scope.
+Infix "+++" := vapp (right associativity, at level 60) : vector_scope.
+
+(* 
+ Local Variables:
+ coq-prog-name: "coqtop.opt -emacs -R . CCP"
+ End:
+*)
